Iris/Iris/ProgramLogic/EctxiLanguage.lean
@@ -13,15 +13,6 @@ open Language.Notation EctxLanguage.Notation FromMathlib
 variable {Expr : Type e}{Val : Type v}{State : Type σ}{Obs : Type o}
 variable {EctxItem : Type i}
 
-class EvContextItem
-    (Expr : Type e)
-    (EctxItem : outParam (Type i)) where
-  fillItem : EctxItem → Expr → Expr
-  fillItem_inj {K} : Function.Injective (fillItem K)
-export EvContextItem (fillItem)
-
-attribute [simp] EvContextItem.fillItem_inj
-
 class EctxItemLanguage
     (Expr     : Type e)
     (EctxItem : outParam <| Type i)
@@ -30,8 +21,10 @@ class EctxItemLanguage
     (Val      : outParam <| Type v)
   extends
     ToVal Expr Val,
-    EvContextItem Expr EctxItem,
+    -- EvContextItem Expr EctxItem,
     BaseStep Expr State Obs where
+  fillItem : EctxItem → Expr → Expr
+  fillItem_inj {K} : Function.Injective (fillItem K)
 
   fillItem_val (e : Expr) (K : EctxItem) :
     (toVal (fillItem K e)).isSome →
@@ -50,133 +43,105 @@ class EctxItemLanguage
     (fillItem Ki e, σ) -<obs>->ᵇ (e', σ', eₜ) →
     (toVal e).isSome
 
+attribute [rocq_alias mixin_fill_item] EctxItemLanguage.fillItem
+attribute [rocq_alias mixin_fill_item_inj] EctxItemLanguage.fillItem_inj
+attribute [rocq_alias mixin_fill_item_val] EctxItemLanguage.fillItem
+attribute [rocq_alias mixin_fill_item_no_val_inj] EctxItemLanguage.fillItem_no_val_inj
 
+attribute [simp] EctxItemLanguage.fillItem_inj
+attribute [grind →] EctxItemLanguage.fillItem_val
+attribute [grind →] EctxItemLanguage.val_stuck
+attribute [grind →] EctxItemLanguage.base_ctx_step_val
 
 namespace EctxItemLanguage
 
 variable [Λ : EctxItemLanguage Expr EctxItem State Obs Val]
 
-abbrev Ectx [EvContext Expr EctxItem] := List EctxItem
+abbrev Ectx [EctxItemLanguage Expr EctxItem State Obs Val] := List EctxItem
 
-instance [EctxItemLanguage Expr EctxItem State Obs Val]:  EvContext Expr (List EctxItem) where
+@[grind]
+instance [Λ : EctxItemLanguage Expr EctxItem State Obs Val] :
+    EvContext Expr Λ.Ectx where
   comp x y := y ++ x
   empty := []
   fill K e := K.foldl (fun x y => fillItem y x) e
   fill_empty (e : Expr) := List.foldl_nil
   fill_comp K₁ K₂ (e : Expr) := Eq.symm List.foldl_append
   fill_inj {K} x y := by
-    induction K generalizing x y with
-    | nil => simp only [List.foldl_nil, imp_self]
-    | cons hd tl IH =>
-      simp at IH ⊢
-      intro sh
-      replace sh := IH _ _ sh
-      simpa only [EvContextItem.fillItem_inj, Function.Injective.eq_iff] using sh
+    induction K generalizing x y <;> grind only [= List.foldl_nil, = List.foldl_cons, !fillItem_inj]
 
 export EvContext (fill)
 
-@[rocq_alias fill_app]
-theorem fill_append (K1 K2 : List EctxItem) (e : Expr) :
-    fill (K1 ++ K2) e = fill K2 (fill K1 e) := by
-  dsimp [fill]
-  grind
+section SelectedGrindRflLemmas
 
-@[elab_as_elim] -- TODO: Properly more this from mathlib
-def reverseRec {motive : List α → Sort _} (nil : motive [])
-    (append_singleton : ∀ (l : List α) (a : α), motive l → motive (l ++ [a])) : ∀ l, motive l
-  | [] => nil
-  | x :: xs => by
-    have := List.eq_nil_or_concat (x :: xs)
-    cases this
-    case inl h => simp at h
-    case inr h =>
-      obtain ⟨init, l, h⟩ := h
-      rw [h]
-      have := reverseRec nil append_singleton init
-      have := append_singleton init l this
-      simpa
-termination_by l => l.length
-decreasing_by
-  simp at h
-  calc init.length
-    _ < (init ++ [l]).length := by grind
-    _ = (x :: xs).length := by grind
+@[grind =, simp]
+theorem fill_cons Ki K (e : Expr) : fill (Ki :: K) e = fill K (fillItem Ki e) := rfl
 
+@[grind =, simp]
+theorem fill_nil (e : Expr) : fill [] e = e := rfl
+
+end SelectedGrindRflLemmas
+
+@[rocq_alias fill_app, grind =, simp]
+theorem fill_append (K1 K2 : Λ.Ectx) (e : Expr) :
+    fill (K1 ++ K2) e = fill K2 (fill K1 e) :=
+  EvContext.fill_comp K2 K1 e |>.symm
+
+@[grind →]
 theorem fill_val K (e : Expr) :
     (toVal (fill K e)).isSome = true → (toVal e).isSome = true := by
-  induction K generalizing e with
-  | nil =>
-    dsimp [fill]
-    grind only
-  | cons init last IH =>
-    simp only [fill, List.foldl_cons] at IH ⊢
-    grind [fill, fillItem_val]
+  induction K generalizing e <;> grind [fillItem_val]
 
-theorem fill_not_val K (e : Expr) :
-     (toVal e) = none → (toVal (fill K e)) = none := by
-  grind [fill_val, Option.isSome_iff_ne_none]
+-- NOTE: Would it be worth having an `isVal` predicate for `Expr`, basically defined
+-- as `toVal e |>.isSome`, so that we could rephrase all instances of `(toVal e).isSome`
+-- as `isVal e` and `toVal e = none` as `¬ isVal e`. That way tactics like `grind` would
+-- be able to match on `toVal`, since as it stands `grind` patterns cannot include `=`,
+-- which means `toVal e = none` is not as well supported.
 
-instance : EctxLanguage Expr (List EctxItem) State Obs Val where
+instance : EctxLanguage Expr Λ.Ectx State Obs Val where
   fill_val K e := fill_val K e
   step_by_val := by
     intros K K' e₁ e₁' σ₁ obs e₂ σ₂ eₜ hfill hred hstep
-    induction K using reverseRec generalizing K' e₁ e₂ with
+    induction K using List.reverseRec generalizing K' e₁ e₂ with
     | nil =>
       simp only [comp, List.append_nil, exists_eq']
     | append_singleton Ks Ki IH =>
-      simp [comp]
-      simp [fill] at hfill
-      cases K' using reverseRec
-      · simp at hfill
+      simp only [comp]
+      cases K' using List.reverseCases with
+      | nil =>
+        simp only [fill_append, fill_cons, fill_nil] at hfill
         subst hfill
         replace hstep := base_ctx_step_val hstep |> fill_val _ _
         grind
-      case append_singleton Ks' Ki' trash =>
-      simp at *
-      have heq : Ki = Ki' := by
-        apply Λ.fillItem_no_val_inj Ki Ki' _ _ hfill
-        · apply fill_not_val
-          assumption
-        · apply fill_not_val
-          apply val_stuck
-          assumption
-      subst heq
-      simp [Function.Injective.eq_iff] at hfill
-      simp [fill] at IH
-      obtain ⟨K'', rfl⟩ := IH hfill hred hstep
-      exists K''
-      simp [comp]
+      | append_singleton Ks' Ki' =>
+        simp only [fill_append, fill_cons, fill_nil] at hfill
+        obtain rfl : Ki = Ki' := by
+          apply fillItem_no_val_inj Ki Ki' _ _ hfill <;> grind [fill_val, Option.isSome_iff_ne_none]
+        simp only [fillItem_inj, Function.Injective.eq_iff] at hfill
+        obtain ⟨K'', rfl⟩ := IH hfill hred hstep
+        exists K''
+        simp [comp]
   val_stuck {e σ obs e' σ' eₜ} := val_stuck
   base_ctx_step_val {K e σ₁ obs e₂ σ₂ eₜ} := by
-    cases K using reverseRec
-    case nil =>
-      simp [empty]
-    case append_singleton init last IH =>
-      intro bstep
-      left
-      simp [fill_append] at *
-      apply fill_val
-      apply base_ctx_step_val
-      assumption
+    cases K using List.reverseRec <;> grind
 
 theorem fill_no_val K (e : Expr) :
     toVal e = none →
     toVal (fill K e) = none := by
-  grind [fill_val]
+  grind only [=> EctxLanguage.fill_not_val]
 
+-- TODO: I don't like that this has the same name as the property it's proving.
+-- It makes it confusing...
 theorem subredexesAreValues (e : Expr) :
     (∀ Ki e', e = fillItem Ki e' → (toVal e').isSome) →
     EctxLanguage.subredexesAreValues e := by
   rintro hsub K e' rfl
-  cases K using reverseRec
+  cases K using List.reverseRec
   case nil => simp [empty]
   case append_singleton init last IH =>
-    simp [empty, Option.ne_none_iff_exists]
-    suffices isSome : (toVal e').isSome from by
-      grind [Option.isSome_iff_exists]
-    apply fill_val
-    apply hsub
-    simp [fill]
-    rfl
+    simp only [empty, List.append_eq_nil_iff, List.cons_ne_self, and_false, imp_false]
+    simp only [Option.ne_none_iff_exists', ←Option.isSome_iff_exists]
+    simp only [fill_append, fill_cons, fill_nil] at hsub
+    grind only [→ fill_val]
 
 end EctxItemLanguage
